verif_LZC.v
@@ -7,10 +7,11 @@ Require Import Stdlib.Strings.Byte.
 Instance CompSpecs : compspecs. make_compspecs prog. Defined.
 Definition Vprog : varspecs. mk_varspecs prog. Defined.
 
+(* Adapted from: https://github.com/PrincetonUniversity/VST/blob/master/progs/verif_queue.v *)
 Definition surely_malloc_spec :=
   DECLARE _surely_malloc
     WITH t:type, gv: globals
-    PRE [ tuint ]
+    PRE [ tulong ]
       PROP (0 <= sizeof t <= Int64.max_unsigned;
             complete_legal_cosu_type t = true;
             natural_aligned natural_alignment t = true)
@@ -20,4 +21,219 @@ Definition surely_malloc_spec :=
       PROP ()
       RETURN (p)
       SEP (mem_mgr gv; malloc_token Ews t p * data_at_ Ews t p).
+
+
+Definition bytes_to_vals (bs : list byte) : list val :=
+  map Vbyte (map Byte.repr (map Z.of_nat (map to_nat bs))).
+
+Definition encode_length_spec :=
+  DECLARE _encode_length
+    WITH sh: share, len: Z, out_: val, out: list val, out_len: Z, gv: globals
+    PRE [ tulong, tptr tuchar ]
+      PROP (writable_share sh; 0 <= len <= Int64.max_unsigned; isptr out_;
+            Zlength (nat_to_bytes (Z.to_nat len)) <= out_len; 0 <= out_len)
+      PARAMS (Vlong (Int64.repr len); out_) GLOBALS (gv)
+      SEP (mem_mgr gv)
+    POST [ tulong ] EX idx: Z,
+      PROP (idx = Zlength (nat_to_bytes (Z.to_nat len)))
+      RETURN (Vlong (Int64.repr idx))
+      SEP (mem_mgr gv;
+           data_at sh (tarray tuchar idx) (bytes_to_vals (nat_to_bytes (Z.to_nat len))) out_).
+
+Definition decode_length_spec :=
+  DECLARE _decode_length
+    WITH sh_in: share, in_: val, in_bytes: list byte, in_len: Z,
+         sh_out: share, out_: val, gv: globals
+    PRE [ tptr tuchar, tulong, tptr tulong ]
+      PROP (readable_share sh_in; writable_share sh_out;
+            0 <= in_len <= 9; (* HERE IS THE ASSUMPTION. *)
+            in_len = Zlength in_bytes)
+      PARAMS (in_; Vlong (Int64.repr in_len); out_) GLOBALS (gv)
+      SEP (mem_mgr gv;
+           data_at sh_in (tarray tuchar in_len) (bytes_to_vals in_bytes) in_;
+           data_at sh_out tulong (Vlong Int64.zero) out_)
+    POST [ tulong ] EX idx: Z,
+      PROP (idx = Zlength (nat_to_bytes (fst (bytes_to_nat in_bytes))); 0 <= idx <= in_len)
+      RETURN (Vlong (Int64.repr idx))
+      SEP (mem_mgr gv;
+           data_at sh_out tulong (Vlong (Int64.repr (Z.of_nat (fst (bytes_to_nat in_bytes))))) out_).
+
+
+Definition find_largest_match_spec :=
+  DECLARE _find_largest_match
+    WITH sh: share, in_: val, in_bytes: list byte, in_len: Z,
+         p: Z, len_: val, off_: val, gv: globals
+    PRE [ tptr tuchar, tulong, tulong, tptr tulong, tptr tulong ]
+      PROP (readable_share sh;
+            0 <= p <= in_len;
+            in_len = Zlength in_bytes;
+            in_len <= Int64.max_unsigned)
+      PARAMS (in_; Vlong (Int64.repr in_len); Vlong (Int64.repr p); len_; off_) GLOBALS (gv)
+      SEP (mem_mgr gv; data_at sh (tarray tuchar in_len) (bytes_to_vals in_bytes) in_)
+    POST [ tvoid ]
+      let result := find_largest_match (slice 0 (Z.to_nat p) in_bytes)
+                                       (slice (Z.to_nat p) (length in_bytes) in_bytes) in
+      PROP () RETURN ()
+      SEP (mem_mgr gv;
+           data_at Ews tulong
+             (Vlong (Int64.repr (Z.of_nat
+               (match result with
+                | Some (len, _) => len
+                | None => 0
+                end)))) len_;
+           data_at Ews tulong
+             (Vlong (Int64.repr (Z.of_nat
+               (match result with
+                | Some (_, off) => off
+                | None => 0
+                end)))) off_).
+
+
+Definition compress_out_size (in_len : Z) : Z :=
+  (9 * in_len + 7) / 8 + 65.
+
+Definition compress_spec :=
+  DECLARE _compress
+    WITH sh: share, in_: val, in_bytes: list byte, in_len: Z, gv: globals
+    PRE [ tptr tuchar, tulong ]
+      PROP (readable_share sh;
+            0 <= in_len <= Int64.max_unsigned;
+            in_len = Zlength in_bytes)
+      PARAMS (in_; Vlong (Int64.repr in_len)) GLOBALS (gv)
+      SEP (mem_mgr gv; data_at sh (tarray tuchar in_len) (bytes_to_vals in_bytes) in_)
+    POST [ tptr tuchar ] EX p: val,
+      let out_bytes := compress_to_bytes in_bytes in
+      PROP (Zlength out_bytes <= compress_out_size in_len)
+      RETURN (p)
+      SEP (mem_mgr gv;
+           malloc_token Ews (tarray tuchar (compress_out_size in_len)) p *
+           data_at Ews (tarray tuchar (Zlength out_bytes)) (bytes_to_vals out_bytes) p).
+
+Definition decompress_spec :=
+  DECLARE _decompress
+    WITH sh: share, in_: val, in_bytes: list byte, in_len: Z, gv: globals
+    PRE [ tptr tuchar, tulong ]
+      PROP (readable_share sh;
+            0 <= in_len <= Int64.max_unsigned;
+            in_len = Z.of_nat (length in_bytes);
+            exists src : list byte,
+              in_bytes = compress_to_bytes src /\ Zlength src <= Int64.max_unsigned)
+      PARAMS (in_; Vlong (Int64.repr in_len)) GLOBALS (gv)
+      SEP (mem_mgr gv; data_at sh (tarray tuchar in_len) (bytes_to_vals in_bytes) in_)
+    POST [ tptr tuchar ] EX p: val,
+      let out_bytes := decompress_from_bytes in_bytes in
+      PROP ()
+      RETURN (p)
+      SEP (mem_mgr gv;
+           data_at sh (tarray tuchar in_len) (bytes_to_vals in_bytes) in_;
+           malloc_token Ews (tarray tuchar (Zlength out_bytes)) p *
+           data_at Ews (tarray tuchar (Zlength out_bytes)) (bytes_to_vals out_bytes) p).
+
+
+Definition Gprog: funspecs :=
+        ltac:(with_library prog [surely_malloc_spec;
+                                 encode_length_spec;
+                                 decode_length_spec;
+                                 find_largest_match_spec;
+                                 compress_spec;
+                                 decompress_spec]).
+
+
+(* Adapted from: https://github.com/PrincetonUniversity/VST/blob/master/progs/verif_queue.v *)
+Lemma body_surely_malloc:
+  semax_body Vprog Gprog f_surely_malloc surely_malloc_spec.
+Proof.
+  start_function.
+  forward_call (* p = malloc(n); *)
+     (t, gv).
+  Intros p.
+  forward_if
+  (PROP ( )
+   LOCAL (temp _p p)
+   SEP (mem_mgr gv; malloc_token Ews t p * data_at_ Ews t p)).
+   - if_tac.
+     + subst p. entailer!.
+     + entailer!.
+   - forward_call 1.
+     contradiction.
+   - if_tac.
+     + contradiction.
+     + Intros. forward. entailer!.
+   - forward. Exists p. entailer!.
+Qed.
+
+
+Lemma encode_length_body:
+  semax_body Vprog Gprog f_encode_length encode_length_spec.
+Proof.
+  start_function.
+  forward_if.
+  - forward.
+    assert (len = 0). {
+      assert (Int64.unsigned (Int64.repr len) = len). {
+        rewrite Int64.unsigned_repr_eq.
+        rewrite Z.mod_small; [reflexivity | rep_lia].
+      }
+      rewrite H3 in H4.
+      auto.
+    }
+    Exists 0.
+    entailer!!.
+    rewrite data_at_tuchar_zero_array_eq; auto.
+  - forward.
+    (* forward_loop ??? *)
+Admitted.
+
+Lemma decode_length_body:
+  semax_body Vprog Gprog f_decode_length decode_length_spec.
+Proof.
+  start_function.
+  forward_if.
+  - forward.
+    forward.
+    assert (Zlength in_bytes = 0). {
+      assert (Int64.unsigned (Int64.repr (Zlength in_bytes)) = (Zlength in_bytes)). {
+        rewrite Int64.unsigned_repr_eq.
+        rewrite Z.mod_small; [reflexivity | rep_lia].
+      }
+      rewrite H1 in H6.
+      auto.
+    }
+    assert (in_bytes = []) by now apply Zlength_nil_inv.
+    unfold nat_to_bytes.
+    subst. simpl.
+    Exists 0.
+    entailer!!.
+    rewrite H6. 
+    unfold bytes_to_vals. simpl.
+    rewrite data_at_tuchar_zero_array_eq; auto.
+  - forward.
+    (* forward_while ??? *)
+Admitted.
+
+
+Lemma find_largest_match_body: 
+  semax_body Vprog Gprog f_find_largest_match find_largest_match_spec.
+Proof.
+  start_function.
+  forward. forward. forward.
+  (* forward_if ??? *)
+Admitted.
+
+
+Lemma compress_body:
+  semax_body Vprog Gprog f_compress compress_spec.
+Proof.
+  start_function.
+  forward.
+  (* forward_call ??? *)
+Admitted.
+
+Lemma decompress_body:
+  semax_body Vprog Gprog f_decompress decompress_spec.
+Proof.
+  start_function.
+  forward.
+  (* forward_call ??? *)
+Admitted.
 
